updates

generic/Zeta.GenericVerifier.fsti
@@ -1,6 +1,8 @@
 module Zeta.GenericVerifier
 
+open Zeta.App
 open Zeta.Time
+open Zeta.Record
 
 (*
  * Verifier built-in methods
@@ -12,7 +14,7 @@ open Zeta.Time
  * These are different from application methods that implement application-specific
  * state machine transitions.
  *)
-type builtin_method =
+type builtin =
   | AddM                    (* Add a record using Merkle verification *)
   | EvictM                  (* Evict a record, while protecting it using Merkle *)
   | AddB                    (* Add a record using Blum verification *)
@@ -21,8 +23,82 @@ type builtin_method =
   | NextEpoch               (* Transition the verifier thread clock to next epoch *)
   | VerifyEpoch             (* *)
 
-noeq type verifier_spec =
-  | VSpec: vtls: Type0 ->                             (* type of thread local state *)
-           valid: (vtls -> bool) ->                   (* valid function indicating if the thread is in a valid state *)
-           clock: (v: vtls {valid v} -> timestamp) -> (* for valid states, the clock of the verifier thread *)
-           verifier_spec
+(* subset of builtins that add a record *)
+let is_add m =
+  match m with
+  | AddM
+  | AddB -> true
+  | _ -> false
+
+(* subset of builtins that evict a record *)
+let is_evict m =
+  match m with
+  | EvictM
+  | EvictB
+  | EvictBM -> true
+  | _ -> false
+
+(* subset of builtins that manage epochs *)
+let is_epoch_bookkeeping m =
+  match m with
+  | NextEpoch
+  | VerifyEpoch -> true
+  | _ -> false
+
+(* identifier type for verifier threads *)
+type thread_id = nat
+
+(* The basic "structure" of a verifier specification. We are interested in specifications that
+ * satisfy additional properties as described below. *)
+noeq
+type verifier_spec_base = {
+  (* type of the verifier thread local state *)
+  vtls_t: Type0;
+
+  (* is the verifier state valid? verification failures take the verifier state to an invalid state. *)
+  valid: vtls_t -> bool;
+
+  (* clock of a verifier thread. *)
+  clock: v:vtls_t{valid v} -> timestamp;
+
+  (* thread_id of the verifier thread *)
+  tid: vtls_t -> thread_id;
+
+  (* input parameter types of builtin methods *)
+  param_t: builtin -> eqtype;
+
+  (* implementations of the builtin methods *)
+  impl: b: builtin -> param_t b -> v:vtls_t{valid v} -> vtls_t;
+
+  (* for add-builtins, extract the added record from the parameters *)
+  add_rec: b: builtin {is_add b} -> param_t b -> record;
+
+  (* for evict builtins, extract the evicted record from the parameters and verifier state *)
+  evict_rec: b: builtin {is_evict b} ->
+             p: param_t b ->
+             v:vtls_t{valid v && valid (impl b p v)} ->
+             record;
+
+  app: app_params;
+}
+
+(* clock is monotonic property *)
+let clock_monotonic_prop (verifier: verifier_spec_base) =
+  forall (b: builtin). forall (p: verifier.param_t b). forall (vtls: verifier.vtls_t {verifier.valid vtls}).
+    {:pattern verifier.impl b p vtls }
+    let clock_pre = verifier.clock vtls in
+    let vtls_post = verifier.impl b p vtls in
+    verifier.valid vtls_post ==> (let clock_post = verifier.clock vtls_post in
+                                  clock_pre `ts_leq` clock_post)
+
+(* thread_id is constant *)
+let thread_id_constant_prop (verifier: verifier_spec_base) =
+  forall (b: builtin). forall (p: verifier.param_t b). forall (vtls: verifier.vtls_t {verifier.valid vtls}).
+    {:pattern verifier.impl b p vtls }
+    let tid_pre = verifier.tid vtls in
+    let tid_post = verifier.tid (verifier.impl b p vtls) in
+    tid_pre = tid_post
+
+type verifier_log_entry (verifier: verifier_spec_base) =
+  | Builtin: b: builtin -> p: verifier.param_t b -> verifier_log_entry verifier
+  | App: f: appfn_id verifier.app -> p: appfn_arg f -> verifier_log_entry verifier
