generic/Zeta.App.fsti
@@ -1,0 +1,146 @@
+module Zeta.App
+
+open Zeta.Hash
+open Zeta.Key
+
+type u8 = FStar.UInt8.t
+type u16 = FStar.UInt16.t
+type u32 = FStar.UInt32.t
+type u64 = FStar.UInt64.t
+
+(*
+ * We first define representation for the argument and result types of
+ *   the functions that the verifier supports
+ *
+ * These are representations of the F* types,
+ *   their interpretation is given by the interp_code function
+ *
+ * Note that we encode key and value also
+ *   This allows us to pass around keys and values with other arguments,
+ *   modeling multiple keys etc. using TPair
+ *   For example, see below the representations for vget and vput (vget_sig and vput_sig)
+ *
+ *)
+
+type code =
+  | TUnit
+  | TUInt8
+  | TUInt16
+  | TUInt32
+  | TUInt64
+  //| TKey
+  | TValue
+  | TPair : code -> code -> code
+
+(*
+ * the application data model specifies the codes for key and data.
+ * Currently, the keys are hard-coded to 256 bit vectors.
+ * TODO: Generalize this to arbitrary keys.
+ *)
+noeq type app_data_model =
+  | AppDataModel: value: eqtype -> app_data_model
+
+(* key type of the application *)
+let app_key (adm: app_data_model) =  key
+
+(* value type of the application *)
+let app_value (adm: app_data_model) = AppDataModel?.value adm
+
+(* TODO: uncomment out TKey after the previous todo is completed (key is generalized) *)
+let rec interp_code (adm: app_data_model) (c:code) : eqtype =
+  match c with
+  | TUnit -> unit
+  | TUInt8 -> u8
+  | TUInt16 -> u16
+  | TUInt32 -> u32
+  | TUInt64 -> u64
+  (* | TKey -> app_key adm *)
+  | TValue -> app_value adm
+  | TPair c1 c2 -> interp_code adm c1 & interp_code adm c2
+
+(*
+ * The function table
+ *
+ * Type of function identifiers
+ *)
+type fn_id = u8
+
+(* data value with the option of a null type *)
+type app_value_nullable (adm: app_data_model) =
+  | Null: app_value_nullable adm
+  | DValue: v: app_value adm -> app_value_nullable adm
+
+(* an application record is a key-value pair *)
+type app_record (adm: app_data_model) = app_key adm & app_value_nullable adm
+
+(* the application state *)
+let app_state (adm: app_data_model) = (k: app_key adm) -> app_value_nullable adm
+
+(*
+ * fn_sig is the signature that each function id in the table is mapped to
+ *
+ * It is parametrized by a, the type of the application specific state
+ *
+ * It contains the argument and result type of the function (their codes)
+ *
+ * f is the actual function
+ *   it takes as input an argument of type (interp_code farg_t),
+ *   a store st
+ *     it must be the case that the footprint of f is contained in the store,
+ *   and an application specific state
+ *
+ *   f then returns a result value (of type (interp_code fres_t)), and a new store and app state
+ *)
+type fn_return_code =
+  | Fn_success
+  | Fn_failure
+
+noeq
+type fn_sig (adm: app_data_model) (a:Type) = {
+  (* code of the argument of the function *)
+  farg_t : code;
+
+  (* code encoding the result type of the function *)
+  fres_t : code;
+
+  (*
+   * the actual function that takes in the argument, a list of records
+   * and returns a list of records, a succ/failure, a result, and
+   * new internal state a
+   *)
+  f : arg:interp_code adm farg_t ->
+      list (app_record adm) ->
+      a ->
+      (fn_return_code & interp_code adm fres_t & a & list (app_record adm));
+}
+
+(*
+ * Finally the function table is a map from functions ids to signatures
+ *)
+type fn_tbl (adm: app_data_model) (a:Type) = Map.t fn_id (fn_sig adm a)
+
+(*
+ * The application parameters: an application specific state type and a function table
+ *)
+noeq
+type app_params = {
+  app_int_state: Type;
+  ainit: app_int_state;
+  adm: app_data_model;
+  tbl : fn_tbl adm app_int_state;
+  // keyhashfn: app_key adm -> data_key;
+  valuehashfn: app_value adm -> hash_value
+}
+
+(* the type of valid function ids of an application *)
+let appfn_id (aprm: app_params) = (fid: fn_id {Map.contains aprm.tbl fid})
+
+(* argument type of a function *)
+let appfn_arg (#aprm: app_params) (fid: appfn_id aprm): eqtype =
+  let fnsig = Map.sel aprm.tbl fid in
+  interp_code aprm.adm fnsig.farg_t
+
+(* return type of a function *)
+let appfn_res (#aprm: app_params) (fid: appfn_id aprm): eqtype =
+  let fnsig = Map.sel aprm.tbl fid in
+  interp_code aprm.adm fnsig.fres_t
