generic/Zeta.Hash.fsti
@@ -1,0 +1,9 @@
+module Zeta.Hash
+
+open FStar.BitVector
+
+(* size of a hash value *)
+let hash_size = 256
+
+(* hash value *)
+type hash_value = bv_t hash_size
